\documentclass[12pt]{article}

\usepackage{amsthm}
\usepackage{amsmath}
\usepackage{graphicx}
\usepackage{hyperref}
\usepackage[utf8]{inputenc}

\newtheorem{theorem}{Theorem}

\newcommand{\norm}[1]{\left\lVert#1\right\rVert}

\title{SVM}

\author{osimpson}

\date{2021-04-16}

\begin{document}

\maketitle

\section{Basics}

\begin{theorem}
    The distance between two parallel hyperplanes, $a^Tx=b_1, a^Tx=b_2$ is 
    $\frac{|b_1-b_2|}{\norm{a}}$.
\end{theorem}

\begin{proof}
    Let $p_1$ be a point on the first plane, and let $p_2$ be the point on the
    second plane closest to $p_1$.  The distance between $p_1$ and $p_2$ is the
    distance between the hyperplanes.  This distance is along the normal vector
    which passes through $p_1$ to $p_2$.  The direction of the normal vector is
    $a$.  For a quick proof of this, consider two points $x_1, x_2$ on the 
    hyperplane.  Both points satisfy the equation $a^Tx=b_1$, so we have that 
    $a^T(x_2-x_1)=0$, and since $x_2-x_1$ defines an arbitrary line on the
    hyperplane, $a$ is orthogonal to the hyperplane.  Therefore, a vector orthogonal
    to the hyperplane that goes through $p_1$ to $p_2$ is given by $p_1+a\lambda=p_2$.

    Then $\norm{p_2-p_1} = \norm{p_1+a\lambda - p_1} = |\lambda| \cdot \norm{a}$.
    We can solve for $\lambda$ using the hyperplane equations:
    \begin{equation}
        \begin{split}
            a^T(p_2-p_1) &= b_2-b_1 \\
            a^T(a\lambda) &= b_2-b_1 \\
            \lambda\norm{a}^2 &= b_2-b_1 \\
            \lambda &= \frac{b_2 - b_1}{\norm{a}^2}
        \end{split}
    \end{equation}
    Thus, $\norm{p_2 - p_1} = \frac{|b_2-b_1|}{\norm{a}}$

\end{proof}

\end{document}


